<?xml version="1.0"?>


<!DOCTYPE rdf:RDF [
    <!ENTITY dcterms "http://purl.org/dc/terms/" >
    <!ENTITY lemon "http://lemon-model.net/lemon#" >
    <!ENTITY owl "http://www.w3.org/2002/07/owl#" >
    <!ENTITY dbnary "http://etytree-virtuoso.wmflabs.org/dbnary#" >
    <!ENTITY dbetym "http://etytree-virtuoso.wmflabs.org/dbnaryetymology#" >
    <!ENTITY xsd "http://www.w3.org/2001/XMLSchema#" >
    <!ENTITY rdfs "http://www.w3.org/2000/01/rdf-schema#" >
    <!ENTITY rdf "http://www.w3.org/1999/02/22-rdf-syntax-ns#" >
]>


<rdf:RDF xmlns="http://etytree-virtuoso.wmflabs.org/dbnaryetymology#"
     xml:base="http://etytree-virtuoso.wmflabs.org/dbnaryetymology"
     xmlns:rdf="http://www.w3.org/1999/02/22-rdf-syntax-ns#"
     xmlns:owl="http://www.w3.org/2002/07/owl#"
     xmlns:xsd="http://www.w3.org/2001/XMLSchema#"
     xmlns:dbnary="http://etytree-virtuoso.wmflabs.org/dbnary#"
     xmlns:dbetym="http://etytree-virtuoso.wmflabs.org/dbnaryetymology#"
     xmlns:lemon="http://lemon-model.net/lemon#"
     xmlns:rdfs="http://www.w3.org/2000/01/rdf-schema#">
    <owl:Ontology rdf:about="http://etytree-virtuoso.wmflabs.org/dbnaryetymology">
        <rdfs:label xml:lang="en">DBnary etymology ontology</rdfs:label>
        <rdfs:comment xml:lang="en">A DBnary ontology extension used to represent etymological data extracted from Wiktionary.</rdfs:comment>
        <imports rdf:resource="http://etytree-virtuoso.wmflabs.org/"/>
    </owl:Ontology>
    

    <!--
    ///////////////////////////////////////////////////////////////////////////////////////
    //
    // Object Properties
    //
    ///////////////////////////////////////////////////////////////////////////////////////
     -->    


    <!-- http://etytree-virtuoso.wmflabs.org/dbnaryetymology#etymologicallyEquivalentTo -->

    <owl:ObjectProperty rdf:about="&dbetym;etymologicallyEquivalentTo">
        <rdfs:comment xml:lang="en">The target and the source EtymologyEntries share the same etymological origin. </rdfs:comment>
        <rdfs:range rdf:resource="&lemon;EtymologyEntry"/>
        <rdfs:domain rdf:resource="&lemon;EtymologyEntry"/>
	<!--rdfs:subPropertyOf rdf:resource="&owl;sameAs"/-->
    </owl:ObjectProperty>
    
    <!-- http://etytree-virtuoso.wmflabs.org/dbnaryetymology#etymologicallyDerivesFrom -->

    <owl:ObjectProperty rdf:about="&dbetym;etymologicallyDerivesFrom">
        <rdfs:comment xml:lang="en">The target EtymologyEntry has been extracted from section Derived Terms in Wiktionary. </rdfs:comment>
        <rdfs:range rdf:resource="&lemon;EtymologyEntry"/>
	<rdfs:domain rdf:resource="&lemon;EtymologyEntry"/>
    </owl:ObjectProperty>
    
    <!-- http://etytree-virtuoso.wmflabs.org/dbnaryetymology#etymologicallyRelatedTo -->

    <owl:ObjectProperty rdf:about="&dbetym;etymologicallyRelatedTo">
        <rdfs:comment xml:lang="en">An underspecified etymological relationship between two EtymologyEntries of type: descendant or etymologically equivalent to. </rdfs:comment>
	<rdfs:range rdf:resource="&lemon;EtymologyEntry"/>
        <rdfs:domain rdf:resource="&lemon;EtymologyEntry"/>
    </owl:ObjectProperty>
    


    <!-- 
    ///////////////////////////////////////////////////////////////////////////////////////
    //
    // Classes
    //
    ///////////////////////////////////////////////////////////////////////////////////////
     -->

    


    <!-- http://etytree-virtuoso.wmflabs.org/dbnaryetymology#EtymologyEntry -->

    <owl:Class rdf:about="&dbetym;EtymologyEntry">
        <rdfs:subClassOf rdf:resource="&lemon;LexicalEntry"/>
        <rdfs:comment xml:lang="en">An EtymologyEntry corresponds to a set of Lexical Entries that share the same etymology but that do not necessarily share the same Part Of Speech. E.g. eng:link_n_1 and eng:link_v_1 are distinct lexical entries and the etymology entry eng:link_ety_1 refers to both of them because eng:link_n_1 and eng:link_v_1 share the same etymology from Old English ang:linke.</rdfs:comment>
    </owl:Class>

</rdf:RDF>



<!-- Generated by the OWL API (version 3.5.0) http://owlapi.sourceforge.net -->

