<?xml version="1.0"?>
<rdf:RDF xmlns="http://kaiko.getalp.org/dbnary#"
     xml:base="http://kaiko.getalp.org/dbnary"
     xmlns:dc="http://purl.org/dc/elements/1.1/"
     xmlns:ns="http://creativecommons.org/ns#"
     xmlns:qb="http://purl.org/linked-data/cube#"
     xmlns:owl="http://www.w3.org/2002/07/owl#"
     xmlns:rdf="http://www.w3.org/1999/02/22-rdf-syntax-ns#"
     xmlns:xml="http://www.w3.org/XML/1998/namespace"
     xmlns:xsd="http://www.w3.org/2001/XMLSchema#"
     xmlns:foaf="http://xmlns.com/foaf/0.1/"
     xmlns:lime="http://www.w3.org/ns/lemon/lime#"
     xmlns:rdfs="http://www.w3.org/2000/01/rdf-schema#"
     xmlns:skos="http://www.w3.org/2004/02/skos/core#"
     xmlns:vann="http://purl.org/vocab/vann/"
     xmlns:void="http://rdfs.org/ns/void#"
     xmlns:dbnary="http://kaiko.getalp.org/dbnary#"
     xmlns:synsem="http://www.w3.org/ns/lemon/synsem#"
     xmlns:dcterms="http://purl.org/dc/terms/"
     xmlns:ontolex="http://www.w3.org/ns/lemon/ontolex#"
     xmlns:vartrans="http://www.w3.org/ns/lemon/vartrans#">
    <owl:Ontology rdf:about="http://kaiko.getalp.org/dbnary">
        <owl:versionIRI rdf:resource="http://kaiko.getalp.org/dbnary/2.1.0"/>
        <owl:imports rdf:resource="http://purl.org/linked-data/cube"/>
        <owl:imports rdf:resource="http://www.w3.org/1999/02/22-rdf-syntax-ns#"/>
        <owl:imports rdf:resource="http://www.w3.org/ns/lemon/lime"/>
        <owl:imports rdf:resource="http://www.w3.org/ns/lemon/ontolex"/>
        <owl:imports rdf:resource="http://www.w3.org/ns/lemon/synsem"/>
        <owl:imports rdf:resource="http://www.w3.org/ns/lemon/vartrans"/>
        <rdfs:comment xml:lang="en">DBnary: A lexicon model designed to allow the representation of lexical data extracted from wiktionary language editions (http://www.wiktionary.org/). The dbnary model extends the ontolex model (http://www.w3.org/ns/lemon/ontolex).</rdfs:comment>
        <rdfs:label>dbnary</rdfs:label>
        <rdfs:seeAlso>http://kaiko.getalp.org/about-dbnary/</rdfs:seeAlso>
    </owl:Ontology>
    


    <!-- 
    ///////////////////////////////////////////////////////////////////////////////////////
    //
    // Object Properties
    //
    ///////////////////////////////////////////////////////////////////////////////////////
     -->

    


    <!-- http://kaiko.getalp.org/dbnary#antonym -->

    <owl:ObjectProperty rdf:about="http://kaiko.getalp.org/dbnary#antonym">
        <rdfs:subPropertyOf rdf:resource="http://kaiko.getalp.org/dbnary#topNymProperty"/>
        <rdfs:comment xml:lang="en">An underspecified antonymy relation between LexicalEntities (Lexical entries or Lexical Senses). This relation is used to encode an information available in a lexicon when the linked Lexical Senses are not known. When both source and target of the relation are Lexical Senses, one should use the corresponding LEMON relation. </rdfs:comment>
    </owl:ObjectProperty>
    


    <!-- http://kaiko.getalp.org/dbnary#approximateSynonym -->

    <owl:ObjectProperty rdf:about="http://kaiko.getalp.org/dbnary#approximateSynonym">
        <rdfs:subPropertyOf rdf:resource="http://kaiko.getalp.org/dbnary#topNymProperty"/>
        <rdfs:comment xml:lang="en">An underspecified approximate synonymy relation between LexicalEntities (Lexical entries or Lexical Senses). This relation is used to encode an information available in a lexicon when the linked Lexical Senses are not known. When both source and target of the relation are Lexical Senses, one should use the corresponding LEMON relation. </rdfs:comment>
    </owl:ObjectProperty>
    


    <!-- http://kaiko.getalp.org/dbnary#describes -->

    <owl:ObjectProperty rdf:about="http://kaiko.getalp.org/dbnary#describes">
        <rdfs:domain rdf:resource="http://kaiko.getalp.org/dbnary#Page"/>
        <rdfs:range rdf:resource="http://www.w3.org/ns/lemon/ontolex#LexicalEntry"/>
        <rdfs:comment xml:lang="en">links a vocable to any lexical entry that share the same written form. </rdfs:comment>
    </owl:ObjectProperty>
    


    <!-- http://kaiko.getalp.org/dbnary#gloss -->

    <owl:ObjectProperty rdf:about="http://kaiko.getalp.org/dbnary#gloss">
        <rdfs:domain>
            <owl:Class>
                <owl:unionOf rdf:parseType="Collection">
                    <rdf:Description rdf:about="http://www.w3.org/1999/02/22-rdf-syntax-ns#Statement"/>
                    <rdf:Description rdf:about="http://www.w3.org/ns/lemon/vartrans#Translation"/>
                </owl:unionOf>
            </owl:Class>
        </rdfs:domain>
        <rdfs:range rdf:resource="http://kaiko.getalp.org/dbnary#Gloss"/>
        <rdfs:comment xml:lang="en">A short description of the context (usually a brief definition) under which the subject Translation or Relation is valid</rdfs:comment>
    </owl:ObjectProperty>
    


    <!-- http://kaiko.getalp.org/dbnary#holonym -->

    <owl:ObjectProperty rdf:about="http://kaiko.getalp.org/dbnary#holonym">
        <rdfs:subPropertyOf rdf:resource="http://kaiko.getalp.org/dbnary#topNymProperty"/>
        <rdfs:comment xml:lang="en">An underspecified holonymy relation between LexicalEntities (Lexical entries or Lexical Senses). This relation is used to encode an information available in a lexicon when the linked Lexical Senses are not known. When both source and target of the relation are Lexical Senses, one should use the corresponding LEMON relation. </rdfs:comment>
    </owl:ObjectProperty>
    


    <!-- http://kaiko.getalp.org/dbnary#hypernym -->

    <owl:ObjectProperty rdf:about="http://kaiko.getalp.org/dbnary#hypernym">
        <rdfs:subPropertyOf rdf:resource="http://kaiko.getalp.org/dbnary#topNymProperty"/>
        <rdfs:comment xml:lang="en">An underspecified hypernymy relation between LexicalEntities (Lexical entries or Lexical Senses). This relation is used to encode an information available in a lexicon when the linked Lexical Senses are not known. When both source and target of the relation are Lexical Senses, one should use the corresponding LEMON relation. </rdfs:comment>
    </owl:ObjectProperty>
    


    <!-- http://kaiko.getalp.org/dbnary#hyponym -->

    <owl:ObjectProperty rdf:about="http://kaiko.getalp.org/dbnary#hyponym">
        <rdfs:subPropertyOf rdf:resource="http://kaiko.getalp.org/dbnary#topNymProperty"/>
        <rdfs:comment xml:lang="en">An underspecified hyponymy relation between LexicalEntities (Lexical entries or Lexical Senses). This relation is used to encode an information available in a lexicon when the linked Lexical Senses are not known. When both source and target of the relation are Lexical Senses, one should use the corresponding LEMON relation. </rdfs:comment>
    </owl:ObjectProperty>
    


    <!-- http://kaiko.getalp.org/dbnary#isTranslationOf -->

    <owl:ObjectProperty rdf:about="http://kaiko.getalp.org/dbnary#isTranslationOf">
        <rdfs:domain rdf:resource="http://kaiko.getalp.org/dbnary#Translation"/>
        <rdfs:range>
            <owl:Class>
                <owl:unionOf rdf:parseType="Collection">
                    <rdf:Description rdf:about="http://kaiko.getalp.org/dbnary#Page"/>
                    <rdf:Description rdf:about="http://www.w3.org/ns/lemon/ontolex#LexicalEntry"/>
                    <rdf:Description rdf:about="http://www.w3.org/ns/lemon/ontolex#LexicalSense"/>
                </owl:unionOf>
            </owl:Class>
        </rdfs:range>
        <rdfs:comment xml:lang="en">links the translation information to the Lexical Entity it belongs to.</rdfs:comment>
    </owl:ObjectProperty>
    


    <!-- http://kaiko.getalp.org/dbnary#meronym -->

    <owl:ObjectProperty rdf:about="http://kaiko.getalp.org/dbnary#meronym">
        <rdfs:subPropertyOf rdf:resource="http://kaiko.getalp.org/dbnary#topNymProperty"/>
        <rdfs:comment xml:lang="en">An underspecified meronymy relation between LexicalEntities (Lexical entries or Lexical Senses). This relation is used to encode an information available in a lexicon when the linked Lexical Senses are not known. When both source and target of the relation are Lexical Senses, one should use the corresponding LEMON relation. </rdfs:comment>
    </owl:ObjectProperty>
    


    <!-- http://kaiko.getalp.org/dbnary#observationLanguage -->

    <owl:ObjectProperty rdf:about="http://kaiko.getalp.org/dbnary#observationLanguage">
        <rdfs:domain rdf:resource="http://purl.org/linked-data/cube#Observation"/>
        <rdfs:range rdf:resource="http://purl.org/dc/terms/LinguisticSystem"/>
    </owl:ObjectProperty>
    


    <!-- http://kaiko.getalp.org/dbnary#synonym -->

    <owl:ObjectProperty rdf:about="http://kaiko.getalp.org/dbnary#synonym">
        <rdfs:subPropertyOf rdf:resource="http://kaiko.getalp.org/dbnary#topNymProperty"/>
        <rdfs:comment xml:lang="en">An underspecified synonymy relation between LexicalEntities (Lexical entries or Lexical Senses). This relation is used to encode an information available in a lexicon when the linked Lexical Senses are not known. When both source and target of the relation are Lexical Senses, one should use the corresponding LEMON relation. </rdfs:comment>
    </owl:ObjectProperty>
    


    <!-- http://kaiko.getalp.org/dbnary#targetLanguage -->

    <owl:ObjectProperty rdf:about="http://kaiko.getalp.org/dbnary#targetLanguage">
        <rdf:type rdf:resource="http://www.w3.org/2002/07/owl#FunctionalProperty"/>
        <rdfs:domain rdf:resource="http://kaiko.getalp.org/dbnary#Translation"/>
        <rdfs:range rdf:resource="http://purl.org/dc/terms/LinguisticSystem"/>
        <rdfs:comment xml:lang="en">The target language of a given translation, defined as a Linguistic System.</rdfs:comment>
    </owl:ObjectProperty>
    


    <!-- http://kaiko.getalp.org/dbnary#topNymProperty -->

    <owl:ObjectProperty rdf:about="http://kaiko.getalp.org/dbnary#topNymProperty">
        <rdfs:domain>
            <owl:Class>
                <owl:unionOf rdf:parseType="Collection">
                    <rdf:Description rdf:about="http://kaiko.getalp.org/dbnary#Page"/>
                    <rdf:Description rdf:about="http://www.w3.org/ns/lemon/ontolex#LexicalEntry"/>
                    <rdf:Description rdf:about="http://www.w3.org/ns/lemon/ontolex#LexicalSense"/>
                </owl:unionOf>
            </owl:Class>
        </rdfs:domain>
        <rdfs:range>
            <owl:Class>
                <owl:unionOf rdf:parseType="Collection">
                    <rdf:Description rdf:about="http://kaiko.getalp.org/dbnary#Page"/>
                    <rdf:Description rdf:about="http://www.w3.org/ns/lemon/ontolex#LexicalEntry"/>
                    <rdf:Description rdf:about="http://www.w3.org/ns/lemon/ontolex#LexicalSense"/>
                </owl:unionOf>
            </owl:Class>
        </rdfs:range>
        <rdfs:comment xml:lang="en">An underspecified lexico semantic relation between LexicalEntities (Lexical entry OR Lexical Sense). This relation is used to encode an information available in a lexicon when the linked Lexical Senses are not known. When both source and target of the relation are Lexical Senses, one should use the corresponding LEMON relation. </rdfs:comment>
    </owl:ObjectProperty>
    


    <!-- http://kaiko.getalp.org/dbnary#troponym -->

    <owl:ObjectProperty rdf:about="http://kaiko.getalp.org/dbnary#troponym">
        <rdfs:subPropertyOf rdf:resource="http://kaiko.getalp.org/dbnary#topNymProperty"/>
        <rdfs:comment xml:lang="en">A verb that indicates more precisely the manner of doing something by replacing a verb of a more generalized meaning. E.g.: &quot;Stroll&quot; is a troponym of &quot;walk&quot;, since it involves a slow and relaxed sort of walking.</rdfs:comment>
    </owl:ObjectProperty>
    


    <!-- 
    ///////////////////////////////////////////////////////////////////////////////////////
    //
    // Data properties
    //
    ///////////////////////////////////////////////////////////////////////////////////////
     -->

    


    <!-- http://kaiko.getalp.org/dbnary#extractorVersion -->

    <owl:DatatypeProperty rdf:about="http://kaiko.getalp.org/dbnary#extractorVersion">
        <rdf:type rdf:resource="http://www.w3.org/2002/07/owl#FunctionalProperty"/>
        <rdfs:comment xml:lang="en">The version number of the extraction program used to produce this dataset from the wiktionary dumps.</rdfs:comment>
    </owl:DatatypeProperty>
    


    <!-- http://kaiko.getalp.org/dbnary#partOfSpeech -->

    <owl:DatatypeProperty rdf:about="http://kaiko.getalp.org/dbnary#partOfSpeech">
        <rdfs:domain rdf:resource="http://www.w3.org/ns/lemon/ontolex#LexicalEntry"/>
        <rdfs:range rdf:resource="http://www.w3.org/2001/XMLSchema#string"/>
        <rdfs:comment xml:lang="en">The original part of speech as it was defined in the Wiktionary page. This property takes a String litteral as object.</rdfs:comment>
    </owl:DatatypeProperty>
    


    <!-- http://kaiko.getalp.org/dbnary#rank -->

    <owl:DatatypeProperty rdf:about="http://kaiko.getalp.org/dbnary#rank">
        <rdfs:range rdf:resource="http://www.w3.org/2001/XMLSchema#int"/>
    </owl:DatatypeProperty>
    


    <!-- http://kaiko.getalp.org/dbnary#senseNumber -->

    <owl:DatatypeProperty rdf:about="http://kaiko.getalp.org/dbnary#senseNumber">
        <rdfs:domain rdf:resource="http://www.w3.org/ns/lemon/ontolex#LexicalSense"/>
        <rdfs:range rdf:resource="http://www.w3.org/2001/XMLSchema#string"/>
        <rdfs:comment xml:lang="en">The number of the lexical Sense in the Lexical Entry, as given by Wiktionary. This property takes a String literal as an object.</rdfs:comment>
    </owl:DatatypeProperty>
    


    <!-- http://kaiko.getalp.org/dbnary#targetLanguageCode -->

    <owl:DatatypeProperty rdf:about="http://kaiko.getalp.org/dbnary#targetLanguageCode">
        <rdf:type rdf:resource="http://www.w3.org/2002/07/owl#FunctionalProperty"/>
        <rdfs:domain rdf:resource="http://kaiko.getalp.org/dbnary#Translation"/>
        <rdfs:range rdf:resource="http://www.w3.org/2001/XMLSchema#string"/>
        <rdfs:comment xml:lang="en">The target language of a given translation. This may be used when the dbnary:targetLanguage object property can not be used.</rdfs:comment>
    </owl:DatatypeProperty>
    


    <!-- http://kaiko.getalp.org/dbnary#translationsWithNoGloss -->

    <owl:DatatypeProperty rdf:about="http://kaiko.getalp.org/dbnary#translationsWithNoGloss"/>
    


    <!-- http://kaiko.getalp.org/dbnary#translationsWithSenseNumber -->

    <owl:DatatypeProperty rdf:about="http://kaiko.getalp.org/dbnary#translationsWithSenseNumber">
        <rdfs:subPropertyOf rdf:resource="http://www.w3.org/2002/07/owl#topDataProperty"/>
    </owl:DatatypeProperty>
    


    <!-- http://kaiko.getalp.org/dbnary#translationsWithSenseNumberAndTextualGloss -->

    <owl:DatatypeProperty rdf:about="http://kaiko.getalp.org/dbnary#translationsWithSenseNumberAndTextualGloss"/>
    


    <!-- http://kaiko.getalp.org/dbnary#translationsWithTextualGloss -->

    <owl:DatatypeProperty rdf:about="http://kaiko.getalp.org/dbnary#translationsWithTextualGloss"/>
    


    <!-- http://kaiko.getalp.org/dbnary#usage -->

    <owl:DatatypeProperty rdf:about="http://kaiko.getalp.org/dbnary#usage">
        <rdfs:domain rdf:resource="http://kaiko.getalp.org/dbnary#Translation"/>
        <rdfs:range rdf:resource="http://www.w3.org/2001/XMLSchema#string"/>
        <rdfs:comment xml:lang="en">Usage note that is used to further annotate the target of the translation.</rdfs:comment>
    </owl:DatatypeProperty>
    


    <!-- http://kaiko.getalp.org/dbnary#wiktionaryDumpVersion -->

    <owl:DatatypeProperty rdf:about="http://kaiko.getalp.org/dbnary#wiktionaryDumpVersion"/>
    


    <!-- http://kaiko.getalp.org/dbnary#writtenForm -->

    <owl:DatatypeProperty rdf:about="http://kaiko.getalp.org/dbnary#writtenForm">
        <rdfs:domain rdf:resource="http://kaiko.getalp.org/dbnary#Translation"/>
        <rdfs:range rdf:resource="http://www.w3.org/2001/XMLSchema#string"/>
        <rdfs:comment xml:lang="en">The written form of a translation equivalent.</rdfs:comment>
    </owl:DatatypeProperty>
    


    <!-- 
    ///////////////////////////////////////////////////////////////////////////////////////
    //
    // Classes
    //
    ///////////////////////////////////////////////////////////////////////////////////////
     -->

    


    <!-- http://kaiko.getalp.org/ObservationLanguageComponent -->

    <owl:Class rdf:about="http://kaiko.getalp.org/ObservationLanguageComponent">
        <rdfs:subClassOf rdf:resource="http://kaiko.getalp.org/dbnary#ObservationComponent"/>
    </owl:Class>
    


    <!-- http://kaiko.getalp.org/TranslationsWithNoGlossComponent -->

    <owl:Class rdf:about="http://kaiko.getalp.org/TranslationsWithNoGlossComponent">
        <rdfs:subClassOf rdf:resource="http://kaiko.getalp.org/dbnary#ObservationComponent"/>
    </owl:Class>
    


    <!-- http://kaiko.getalp.org/TranslationsWithSenseNumberAndTextualGlossComponent -->

    <owl:Class rdf:about="http://kaiko.getalp.org/TranslationsWithSenseNumberAndTextualGlossComponent">
        <rdfs:subClassOf rdf:resource="http://kaiko.getalp.org/dbnary#ObservationComponent"/>
    </owl:Class>
    


    <!-- http://kaiko.getalp.org/TranslationsWithSenseNumberComponent -->

    <owl:Class rdf:about="http://kaiko.getalp.org/TranslationsWithSenseNumberComponent">
        <rdfs:subClassOf rdf:resource="http://kaiko.getalp.org/dbnary#ObservationComponent"/>
    </owl:Class>
    


    <!-- http://kaiko.getalp.org/TranslationsWithTextualGlossComponent -->

    <owl:Class rdf:about="http://kaiko.getalp.org/TranslationsWithTextualGlossComponent">
        <rdfs:subClassOf rdf:resource="http://kaiko.getalp.org/dbnary#ObservationComponent"/>
    </owl:Class>
    


    <!-- http://kaiko.getalp.org/WiktionaryDumpVersionComponent -->

    <owl:Class rdf:about="http://kaiko.getalp.org/WiktionaryDumpVersionComponent">
        <rdfs:subClassOf rdf:resource="http://kaiko.getalp.org/dbnary#ObservationComponent"/>
    </owl:Class>
    


    <!-- http://kaiko.getalp.org/dbnary#Gloss -->

    <owl:Class rdf:about="http://kaiko.getalp.org/dbnary#Gloss">
        <rdfs:comment xml:lang="en">A gloss used to represent the context in which a translation or a relation is valid.</rdfs:comment>
    </owl:Class>
    


    <!-- http://kaiko.getalp.org/dbnary#ObservationComponent -->

    <owl:Class rdf:about="http://kaiko.getalp.org/dbnary#ObservationComponent"/>
    


    <!-- http://kaiko.getalp.org/dbnary#Page -->

    <owl:Class rdf:about="http://kaiko.getalp.org/dbnary#Page">
        <rdfs:comment xml:lang="en">A Page corresponds to a Wiktionary web page describing a set of Lexical Entries that usually share the same written form but that do not necessarily share the same Part Of Speech. E.g. cat_n and cat_v are distinct lexical entries while the page &quot;cat&quot; refers to both of them.</rdfs:comment>
    </owl:Class>
    


    <!-- http://kaiko.getalp.org/dbnary#Translation -->

    <owl:Class rdf:about="http://kaiko.getalp.org/dbnary#Translation">
        <rdfs:subClassOf rdf:resource="http://www.w3.org/2002/07/owl#Thing"/>
        <rdfs:comment xml:lang="en">Describe translation information for a Lexical Entry or a Lexical Sense.</rdfs:comment>
    </owl:Class>
    


    <!-- http://purl.org/dc/terms/LinguisticSystem -->

    <owl:Class rdf:about="http://purl.org/dc/terms/LinguisticSystem"/>
    


    <!-- 
    ///////////////////////////////////////////////////////////////////////////////////////
    //
    // Individuals
    //
    ///////////////////////////////////////////////////////////////////////////////////////
     -->

    


    <!-- http://kaiko.getalp.org/ObservationLanguageComponent -->

    <owl:NamedIndividual rdf:about="http://kaiko.getalp.org/ObservationLanguageComponent">
        <rdf:type rdf:resource="http://purl.org/linked-data/cube#ComponentSpecification"/>
        <qb:dimension rdf:resource="http://kaiko.getalp.org/dbnary#observationLanguage"/>
    </owl:NamedIndividual>
    


    <!-- http://kaiko.getalp.org/TranslationsWithNoGlossComponent -->

    <owl:NamedIndividual rdf:about="http://kaiko.getalp.org/TranslationsWithNoGlossComponent">
        <rdf:type rdf:resource="http://purl.org/linked-data/cube#ComponentSpecification"/>
        <qb:measure rdf:resource="http://kaiko.getalp.org/dbnary#translationsWithNoGloss"/>
    </owl:NamedIndividual>
    


    <!-- http://kaiko.getalp.org/TranslationsWithSenseNumberAndTextualGlossComponent -->

    <owl:NamedIndividual rdf:about="http://kaiko.getalp.org/TranslationsWithSenseNumberAndTextualGlossComponent">
        <rdf:type rdf:resource="http://purl.org/linked-data/cube#ComponentSpecification"/>
        <qb:measure rdf:resource="http://kaiko.getalp.org/dbnary#translationsWithSenseNumberAndTextualGloss"/>
    </owl:NamedIndividual>
    


    <!-- http://kaiko.getalp.org/TranslationsWithSenseNumberComponent -->

    <owl:NamedIndividual rdf:about="http://kaiko.getalp.org/TranslationsWithSenseNumberComponent">
        <rdf:type rdf:resource="http://purl.org/linked-data/cube#ComponentSpecification"/>
        <qb:measure rdf:resource="http://kaiko.getalp.org/dbnary#translationsWithSenseNumber"/>
    </owl:NamedIndividual>
    


    <!-- http://kaiko.getalp.org/TranslationsWithTextualGlossComponent -->

    <owl:NamedIndividual rdf:about="http://kaiko.getalp.org/TranslationsWithTextualGlossComponent">
        <rdf:type rdf:resource="http://purl.org/linked-data/cube#ComponentSpecification"/>
        <qb:measure rdf:resource="http://kaiko.getalp.org/dbnary#translationsWithTextualGloss"/>
    </owl:NamedIndividual>
    


    <!-- http://kaiko.getalp.org/WiktionaryDumpVersionComponent -->

    <owl:NamedIndividual rdf:about="http://kaiko.getalp.org/WiktionaryDumpVersionComponent">
        <rdf:type rdf:resource="http://purl.org/linked-data/cube#ComponentSpecification"/>
        <qb:dimension rdf:resource="http://kaiko.getalp.org/dbnary#wiktionaryDumpVersion"/>
    </owl:NamedIndividual>
    


    <!-- http://kaiko.getalp.org/dbnary#observationLanguage -->

    <owl:NamedIndividual rdf:about="http://kaiko.getalp.org/dbnary#observationLanguage">
        <rdf:type rdf:resource="http://purl.org/linked-data/cube#MeasureProperty"/>
    </owl:NamedIndividual>
    


    <!-- http://kaiko.getalp.org/dbnary#translationGlossesCube -->

    <owl:NamedIndividual rdf:about="http://kaiko.getalp.org/dbnary#translationGlossesCube">
        <rdf:type rdf:resource="http://purl.org/linked-data/cube#DataSet"/>
        <qb:structure rdf:resource="http://kaiko.getalp.org/dbnary#translationGlossesDataStructure"/>
        <rdfs:comment xml:lang="en">The Data Cube containing observations of translations and their associated glosses.</rdfs:comment>
    </owl:NamedIndividual>
    


    <!-- http://kaiko.getalp.org/dbnary#translationGlossesDataStructure -->

    <owl:NamedIndividual rdf:about="http://kaiko.getalp.org/dbnary#translationGlossesDataStructure">
        <rdf:type rdf:resource="http://purl.org/linked-data/cube#DataStructureDefinition"/>
        <qb:component rdf:resource="http://kaiko.getalp.org/ObservationLanguageComponent"/>
        <qb:component rdf:resource="http://kaiko.getalp.org/TranslationsWithNoGlossComponent"/>
        <qb:component rdf:resource="http://kaiko.getalp.org/TranslationsWithSenseNumberAndTextualGlossComponent"/>
        <qb:component rdf:resource="http://kaiko.getalp.org/TranslationsWithSenseNumberComponent"/>
        <qb:component rdf:resource="http://kaiko.getalp.org/TranslationsWithTextualGlossComponent"/>
        <qb:component rdf:resource="http://kaiko.getalp.org/WiktionaryDumpVersionComponent"/>
        <rdfs:comment xml:lang="en">The DataStructure of the DataCube describing the translations and their associated glosses</rdfs:comment>
    </owl:NamedIndividual>
    


    <!-- http://kaiko.getalp.org/dbnary#translationsWithNoGloss -->

    <owl:NamedIndividual rdf:about="http://kaiko.getalp.org/dbnary#translationsWithNoGloss">
        <rdf:type rdf:resource="http://purl.org/linked-data/cube#MeasureProperty"/>
    </owl:NamedIndividual>
    


    <!-- http://kaiko.getalp.org/dbnary#translationsWithSenseNumber -->

    <owl:NamedIndividual rdf:about="http://kaiko.getalp.org/dbnary#translationsWithSenseNumber">
        <rdf:type rdf:resource="http://purl.org/linked-data/cube#MeasureProperty"/>
    </owl:NamedIndividual>
    


    <!-- http://kaiko.getalp.org/dbnary#translationsWithSenseNumberAndTextualGloss -->

    <owl:NamedIndividual rdf:about="http://kaiko.getalp.org/dbnary#translationsWithSenseNumberAndTextualGloss">
        <rdf:type rdf:resource="http://purl.org/linked-data/cube#MeasureProperty"/>
    </owl:NamedIndividual>
    


    <!-- http://kaiko.getalp.org/dbnary#translationsWithTextualGloss -->

    <owl:NamedIndividual rdf:about="http://kaiko.getalp.org/dbnary#translationsWithTextualGloss">
        <rdf:type rdf:resource="http://purl.org/linked-data/cube#MeasureProperty"/>
    </owl:NamedIndividual>
    


    <!-- http://kaiko.getalp.org/dbnary#wiktionaryDumpVersion -->

    <owl:NamedIndividual rdf:about="http://kaiko.getalp.org/dbnary#wiktionaryDumpVersion">
        <rdf:type rdf:resource="http://purl.org/linked-data/cube#DimensionProperty"/>
    </owl:NamedIndividual>
    


    <!-- 
    ///////////////////////////////////////////////////////////////////////////////////////
    //
    // Annotations
    //
    ///////////////////////////////////////////////////////////////////////////////////////
     -->

    <rdf:Description rdf:about="http://kaiko.getalp.org/dbnary#observationLanguage">
        <rdfs:comment xml:lang="en">The language dimension of an observation</rdfs:comment>
    </rdf:Description>
    <rdf:Description rdf:about="http://kaiko.getalp.org/dbnary#translationsWithNoGloss">
        <rdfs:comment xml:lang="en">count of the number of translation that is not associated to a gloss.</rdfs:comment>
    </rdf:Description>
    <rdf:Description rdf:about="http://kaiko.getalp.org/dbnary#translationsWithSenseNumber">
        <rdfs:comment xml:lang="en">count of the number of translations that are associated to a gloss containing only a sense number.</rdfs:comment>
    </rdf:Description>
    <rdf:Description rdf:about="http://kaiko.getalp.org/dbnary#translationsWithSenseNumberAndTextualGloss">
        <rdfs:comment xml:lang="en">count of the number of translations that are associated to a gloss containing both a sense number and a textual description</rdfs:comment>
    </rdf:Description>
    <rdf:Description rdf:about="http://kaiko.getalp.org/dbnary#translationsWithTextualGloss">
        <rdfs:comment xml:lang="en">count of the number of translations that are associated with a gloss containing only a textual description.</rdfs:comment>
    </rdf:Description>
    <rdf:Description rdf:about="http://kaiko.getalp.org/dbnary#wiktionaryDumpVersion">
        <rdfs:comment xml:lang="en">version number of the wiktionary dump from which the lexical data is extracted</rdfs:comment>
    </rdf:Description>
</rdf:RDF>



<!-- Generated by the OWL API (version 4.5.9.2019-02-01T07:24:44Z) https://github.com/owlcs/owlapi -->

