<?xml version="1.0"?>


<!DOCTYPE rdf:RDF [
    <!ENTITY void "http://rdfs.org/ns/void#" >
    <!ENTITY dcterms "http://purl.org/dc/terms/" >
    <!ENTITY vann "http://purl.org/vocab/vann/" >
    <!ENTITY owl "http://www.w3.org/2002/07/owl#" >
    <!ENTITY cc "http://creativecommons.org/ns#" >
    <!ENTITY dc "http://purl.org/dc/elements/1.1/" >
    <!ENTITY xsd "http://www.w3.org/2001/XMLSchema#" >
    <!ENTITY ontolex "http://www.w3.org/ns/lemon/ontolex#" >
    <!ENTITY rdfs "http://www.w3.org/2000/01/rdf-schema#" >
    <!ENTITY rdf "http://www.w3.org/1999/02/22-rdf-syntax-ns#" >
]>


<rdf:RDF xmlns="http://www.w3.org/ns/lemon/lime#"
     xml:base="http://www.w3.org/ns/lemon/lime"
     xmlns:cc="http://creativecommons.org/ns#"
     xmlns:void="http://rdfs.org/ns/void#"
     xmlns:rdf="http://www.w3.org/1999/02/22-rdf-syntax-ns#"
     xmlns:owl="http://www.w3.org/2002/07/owl#"
     xmlns:xsd="http://www.w3.org/2001/XMLSchema#"
     xmlns:dcterms="http://purl.org/dc/terms/"
     xmlns:ontolex="http://www.w3.org/ns/lemon/ontolex#"
     xmlns:rdfs="http://www.w3.org/2000/01/rdf-schema#"
     xmlns:vann="http://purl.org/vocab/vann/"
     xmlns:dc="http://purl.org/dc/elements/1.1/">
    <owl:Ontology rdf:about="http://www.w3.org/ns/lemon/lime">
        <rdfs:label xml:lang="en">Lexicon Model for Ontologies - LIngusitic MEtadata (LIME)</rdfs:label>
        <owl:versionInfo rdf:datatype="&xsd;decimal">1.0</owl:versionInfo>
        <dc:modified rdf:datatype="&xsd;date">2016-01-10</dc:modified>
        <dc:issued rdf:datatype="&xsd;date">2016-01-10</dc:issued>
        <vann:preferredNamespaceUri rdf:datatype="&xsd;string">http://www.w3.org/ns/lemon/lime#</vann:preferredNamespaceUri>
        <vann:preferredNamespacePrefix rdf:datatype="&xsd;string">lime</vann:preferredNamespacePrefix>
        <dc:rights>CC-Zero</dc:rights>
        <dcterms:description xml:lang="en">LIME (LInguistic MEtadata) is a vocabulary for expressing linguistic metadata about linguistic resources and linguistically grounded datasets.</dcterms:description>
        <dcterms:title xml:lang="en">Vocabulary of Linguistic Metadata</dcterms:title>
        <dc:contributor rdf:resource="http://art.uniroma2.it/fiorelli/"/>
        <dc:contributor rdf:resource="http://art.uniroma2.it/stellato/"/>
        <dc:contributor rdf:resource="http://jogracia.url.ph/web/"/>
        <dc:creator rdf:resource="http://john.mccr.ae/"/>
        <dc:contributor rdf:resource="http://mayor2.dia.fi.upm.es/oeg-upm/index.php/en/teachers/52-emontiel"/>
        <dc:creator rdf:resource="http://www.cimiano.de/"/>
        <dc:contributor rdf:resource="http://www.dfki.de/~declerck/"/>
        <dc:contributor rdf:resource="http://www.ilc.cnr.it/en/content/anas-fahad-khan"/>
        <dc:contributor rdf:resource="http://www.istc.cnr.it/people/aldo-gangemi"/>
        <dc:contributor rdf:resource="http://www.oeg-upm.net/index.php/teachers/53-lupe"/>
        <dc:contributor rdf:resource="http://www.paulbuitelaar.net/"/>
        <dc:publisher rdf:resource="http://www.w3.org/community/ontolex"/>
        <owl:imports rdf:resource="http://www.w3.org/ns/lemon/ontolex"/>
        <cc:license rdf:resource="https://creativecommons.org/publicdomain/zero/1.0/"/>
        <dc:contributor rdf:resource="https://sites.google.com/site/francescafrontini/"/>
    </owl:Ontology>
    


    <!-- 
    ///////////////////////////////////////////////////////////////////////////////////////
    //
    // Annotation properties
    //
    ///////////////////////////////////////////////////////////////////////////////////////
     -->

    


    <!-- http://rdfs.org/ns/void#vocabulary -->

    <owl:AnnotationProperty rdf:about="&void;vocabulary"/>
    


    <!-- 
    ///////////////////////////////////////////////////////////////////////////////////////
    //
    // Object Properties
    //
    ///////////////////////////////////////////////////////////////////////////////////////
     -->

    


    <!-- http://rdfs.org/ns/void#subset -->

    <owl:ObjectProperty rdf:about="&void;subset"/>
    


    <!-- http://rdfs.org/ns/void#vocabulary -->

    <owl:ObjectProperty rdf:about="&void;vocabulary"/>
    


    <!-- http://www.w3.org/ns/lemon/lime#conceptualDataset -->

    <owl:ObjectProperty rdf:about="http://www.w3.org/ns/lemon/lime#conceptualDataset">
        <rdfs:label xml:lang="de">Konzeptdatensatz</rdfs:label>
        <rdfs:label xml:lang="en">conceptual dataset</rdfs:label>
        <rdfs:label xml:lang="es">conjunto de conceptos</rdfs:label>
        <rdfs:label xml:lang="fr">banque de concepts</rdfs:label>
        <rdfs:label xml:lang="it">banca concetti</rdfs:label>
        <rdfs:label xml:lang="nl">dataset van begrippen</rdfs:label>
        <rdfs:isDefinedBy>http://www.w3.org/ns/lemon/lime</rdfs:isDefinedBy>
        <rdfs:comment xml:lang="en">The &apos;conceptual dataset&apos; property relates a lexical link set or a conceptualization set to a corresponding concept set.</rdfs:comment>
        <rdfs:range rdf:resource="&ontolex;ConceptSet"/>
        <rdfs:domain>
            <owl:Class>
                <owl:unionOf rdf:parseType="Collection">
                    <rdf:Description rdf:about="http://www.w3.org/ns/lemon/lime#ConceptualizationSet"/>
                    <rdf:Description rdf:about="http://www.w3.org/ns/lemon/lime#LexicalLinkset"/>
                </owl:unionOf>
            </owl:Class>
        </rdfs:domain>
    </owl:ObjectProperty>
    


    <!-- http://www.w3.org/ns/lemon/lime#entry -->

    <owl:ObjectProperty rdf:about="http://www.w3.org/ns/lemon/lime#entry">
        <rdfs:label xml:lang="af">inskrywing</rdfs:label>
        <rdfs:label xml:lang="de">Eintrag</rdfs:label>
        <rdfs:label xml:lang="en">entry</rdfs:label>
        <rdfs:label xml:lang="es">entrada</rdfs:label>
        <rdfs:label xml:lang="fr">entrée</rdfs:label>
        <rdfs:label xml:lang="it">entrata</rdfs:label>
        <rdfs:label xml:lang="nl">Item</rdfs:label>
        <rdfs:label xml:lang="pt">entrada</rdfs:label>
        <rdfs:label xml:lang="ro">înregistrare</rdfs:label>
        <rdfs:label xml:lang="sv">ingång</rdfs:label>
        <rdfs:isDefinedBy>http://www.w3.org/ns/lemon/lime</rdfs:isDefinedBy>
        <rdfs:comment xml:lang="en">The &apos;entry&apos; property relates a lexicon to one of the lexical entries contained in it.</rdfs:comment>
        <rdfs:domain rdf:resource="http://www.w3.org/ns/lemon/lime#Lexicon"/>
        <rdfs:range rdf:resource="&ontolex;LexicalEntry"/>
    </owl:ObjectProperty>
    


    <!-- http://www.w3.org/ns/lemon/lime#lexicalizationModel -->

    <owl:ObjectProperty rdf:about="http://www.w3.org/ns/lemon/lime#lexicalizationModel">
        <rdfs:subPropertyOf rdf:resource="&void;vocabulary"/>
        <rdfs:domain rdf:resource="http://www.w3.org/ns/lemon/lime#LexicalizationSet"/>
    </owl:ObjectProperty>
    


    <!-- http://www.w3.org/ns/lemon/lime#lexiconDataset -->

    <owl:ObjectProperty rdf:about="http://www.w3.org/ns/lemon/lime#lexiconDataset">
        <rdf:type rdf:resource="&owl;FunctionalProperty"/>
        <rdfs:label xml:lang="af">leksikale datastel</rdfs:label>
        <rdfs:label xml:lang="de">Lexikondatensatz</rdfs:label>
        <rdfs:label xml:lang="en">lexicon dataset</rdfs:label>
        <rdfs:label xml:lang="es">conjunto de datos del lexicón</rdfs:label>
        <rdfs:label xml:lang="fr">banque de données lexicales</rdfs:label>
        <rdfs:label xml:lang="it">banca dati lessicale</rdfs:label>
        <rdfs:label xml:lang="nl">lexicale dataset</rdfs:label>
        <rdfs:label xml:lang="ro">set de date de lexicon</rdfs:label>
        <rdfs:label xml:lang="sv">lexikondatamängd</rdfs:label>
        <rdfs:comment xml:lang="en">The &apos;lexicon dataset&apos; property indicates the lexicon that contains the entries refered to in a lexicalization set or a conceptualization set.</rdfs:comment>
        <rdfs:isDefinedBy rdf:resource="http://www.w3.org/ns/lemon/lime"/>
        <rdfs:range rdf:resource="http://www.w3.org/ns/lemon/lime#Lexicon"/>
        <rdfs:domain>
            <owl:Class>
                <owl:unionOf rdf:parseType="Collection">
                    <rdf:Description rdf:about="http://www.w3.org/ns/lemon/lime#ConceptualizationSet"/>
                    <rdf:Description rdf:about="http://www.w3.org/ns/lemon/lime#LexicalizationSet"/>
                </owl:unionOf>
            </owl:Class>
        </rdfs:domain>
    </owl:ObjectProperty>
    


    <!-- http://www.w3.org/ns/lemon/lime#linguisticCatalog -->

    <owl:ObjectProperty rdf:about="http://www.w3.org/ns/lemon/lime#linguisticCatalog">
        <rdfs:label xml:lang="de">linguistische Kategorienmodell</rdfs:label>
        <rdfs:label xml:lang="en">lingustic catalog</rdfs:label>
        <rdfs:label xml:lang="es">conjunto de categoríes lingüísticas</rdfs:label>
        <rdfs:label xml:lang="fr">banque de catégories linguistiques</rdfs:label>
        <rdfs:label xml:lang="it">banca categorie linguistiche</rdfs:label>
        <rdfs:label xml:lang="nl">verzameling van taalkundige categories</rdfs:label>
        <rdfs:comment xml:lang="en">The &apos;linguistic catalog&apos; property indicates the catalog of linguistic categories used in a lexicon to define linguistic properties of lexical entries.</rdfs:comment>
        <rdfs:isDefinedBy>http://www.w3.org/ns/lemon/lime</rdfs:isDefinedBy>
        <rdfs:range rdf:resource="http://purl.org/vocommons/voaf#Vocabulary"/>
        <rdfs:domain rdf:resource="http://www.w3.org/ns/lemon/lime#Lexicon"/>
    </owl:ObjectProperty>
    


    <!-- http://www.w3.org/ns/lemon/lime#partition -->

    <owl:ObjectProperty rdf:about="http://www.w3.org/ns/lemon/lime#partition">
        <rdfs:label xml:lang="de">Teilung</rdfs:label>
        <rdfs:label xml:lang="en">partition</rdfs:label>
        <rdfs:label xml:lang="es">partición</rdfs:label>
        <rdfs:label xml:lang="fr">partition</rdfs:label>
        <rdfs:label xml:lang="it">partizione</rdfs:label>
        <rdfs:label xml:lang="nl">verdeling</rdfs:label>
        <rdfs:comment xml:lang="en">The &apos;partition&apos; property relates a lexicalization set or lexical linkset to a logical subset that contains lexicalizations for a given ontological type only.</rdfs:comment>
        <rdfs:subPropertyOf rdf:resource="&void;subset"/>
        <rdfs:isDefinedBy rdf:resource="http://www.w3.org/ns/lemon/lime"/>
        <rdfs:domain>
            <owl:Class>
                <owl:unionOf rdf:parseType="Collection">
                    <rdf:Description rdf:about="http://www.w3.org/ns/lemon/lime#LexicalLinkset"/>
                    <rdf:Description rdf:about="http://www.w3.org/ns/lemon/lime#LexicalizationSet"/>
                </owl:unionOf>
            </owl:Class>
        </rdfs:domain>
        <rdfs:range>
            <owl:Class>
                <owl:unionOf rdf:parseType="Collection">
                    <rdf:Description rdf:about="http://www.w3.org/ns/lemon/lime#LexicalLinkset"/>
                    <rdf:Description rdf:about="http://www.w3.org/ns/lemon/lime#LexicalizationSet"/>
                </owl:unionOf>
            </owl:Class>
        </rdfs:range>
    </owl:ObjectProperty>
    


    <!-- http://www.w3.org/ns/lemon/lime#referenceDataset -->

    <owl:ObjectProperty rdf:about="http://www.w3.org/ns/lemon/lime#referenceDataset">
        <rdf:type rdf:resource="&owl;FunctionalProperty"/>
        <rdfs:label xml:lang="af">verwysingsdatastel</rdfs:label>
        <rdfs:label xml:lang="de">Referenzdatensatz</rdfs:label>
        <rdfs:label xml:lang="en">reference dataset</rdfs:label>
        <rdfs:label xml:lang="es">conjunto de datos de referencia</rdfs:label>
        <rdfs:label xml:lang="fr">banque de réfèrences</rdfs:label>
        <rdfs:label xml:lang="it">banca riferimenti</rdfs:label>
        <rdfs:label xml:lang="nl">verzameling van referenties</rdfs:label>
        <rdfs:label xml:lang="ro">setul de date de referință</rdfs:label>
        <rdfs:label xml:lang="sv">referensdatamängd</rdfs:label>
        <rdfs:comment xml:lang="en">The &apos;reference dataset&apos; property indicates the dataset that contains the domain objects or vocabulary elements that are either referenced by a given lexicon, providing the grounding vocabulary for the meaning of the lexical entries, or linked to lexical concepts in a concept set by means of a lexical link set.</rdfs:comment>
        <rdfs:range rdf:resource="&void;Dataset"/>
        <rdfs:isDefinedBy rdf:resource="http://www.w3.org/ns/lemon/lime"/>
        <rdfs:domain>
            <owl:Class>
                <owl:unionOf rdf:parseType="Collection">
                    <rdf:Description rdf:about="http://www.w3.org/ns/lemon/lime#LexicalLinkset"/>
                    <rdf:Description rdf:about="http://www.w3.org/ns/lemon/lime#LexicalizationSet"/>
                </owl:unionOf>
            </owl:Class>
        </rdfs:domain>
    </owl:ObjectProperty>
    


    <!-- http://www.w3.org/ns/lemon/lime#resourceType -->

    <owl:ObjectProperty rdf:about="http://www.w3.org/ns/lemon/lime#resourceType">
        <rdf:type rdf:resource="&owl;FunctionalProperty"/>
        <rdfs:label xml:lang="de">Ressourcentyp</rdfs:label>
        <rdfs:label xml:lang="en">resource type</rdfs:label>
        <rdfs:label xml:lang="es">tipo de recurso</rdfs:label>
        <rdfs:label xml:lang="fr">type de ressource</rdfs:label>
        <rdfs:label xml:lang="it">tipo di risorsa</rdfs:label>
        <rdfs:label xml:lang="nl">type van ressource</rdfs:label>
        <rdfs:isDefinedBy>http://www.w3.org/ns/lemon/lime</rdfs:isDefinedBy>
        <rdfs:comment xml:lang="en">The &apos;resource type&apos; property indicates the type of ontological entity of a lexicalization set or lexical linkset.</rdfs:comment>
        <rdfs:range rdf:resource="&rdfs;Class"/>
        <rdfs:domain>
            <owl:Class>
                <owl:unionOf rdf:parseType="Collection">
                    <rdf:Description rdf:about="http://www.w3.org/ns/lemon/lime#LexicalLinkset"/>
                    <rdf:Description rdf:about="http://www.w3.org/ns/lemon/lime#LexicalizationSet"/>
                </owl:unionOf>
            </owl:Class>
        </rdfs:domain>
    </owl:ObjectProperty>
    


    <!-- 
    ///////////////////////////////////////////////////////////////////////////////////////
    //
    // Data properties
    //
    ///////////////////////////////////////////////////////////////////////////////////////
     -->

    


    <!-- http://www.w3.org/ns/lemon/lime#avgAmbiguity -->

    <owl:DatatypeProperty rdf:about="http://www.w3.org/ns/lemon/lime#avgAmbiguity">
        <rdfs:label xml:lang="de">Durchschnittliche Amiguität</rdfs:label>
        <rdfs:label xml:lang="en">average ambiguity</rdfs:label>
        <rdfs:label xml:lang="es">ambigüedad promedia</rdfs:label>
        <rdfs:label xml:lang="fr">ambiguïté moyenne</rdfs:label>
        <rdfs:label xml:lang="it">ambiguità media</rdfs:label>
        <rdfs:label xml:lang="nl">gemiddelde ambiguïteit</rdfs:label>
        <rdfs:comment xml:lang="en">The &apos;average ambiguity&apos; property indicates the average number of lexical concepts evoked by each lemma/canonical form in the lexicon.</rdfs:comment>
        <rdfs:isDefinedBy>http://www.w3.org/ns/lemon/lime</rdfs:isDefinedBy>
        <rdfs:range rdf:resource="&xsd;decimal"/>
        <rdfs:domain rdf:resource="http://www.w3.org/ns/lemon/lime#ConceptualizationSet"/>
    </owl:DatatypeProperty>
    


    <!-- http://www.w3.org/ns/lemon/lime#avgNumOfLexicalizations -->

    <owl:DatatypeProperty rdf:about="http://www.w3.org/ns/lemon/lime#avgNumOfLexicalizations">
        <rdfs:label xml:lang="af">gemiddelde aantal leksikaliserings</rdfs:label>
        <rdfs:label xml:lang="de">Durchschnittliche Anzahl von Lexikalisierungen</rdfs:label>
        <rdfs:label xml:lang="en">average number of lexicalizations</rdfs:label>
        <rdfs:label xml:lang="es">promedio de lexicalizaciones</rdfs:label>
        <rdfs:label xml:lang="fr">nombre moyen de lexicalisations</rdfs:label>
        <rdfs:label xml:lang="it">numero medio di lessicalizzazioni</rdfs:label>
        <rdfs:label xml:lang="nl">gemiddeld aantal van lexicalisatie</rdfs:label>
        <rdfs:label xml:lang="pt">numero medio de lexicalizações</rdfs:label>
        <rdfs:label xml:lang="ro">numărul mediu de lexicalizari</rdfs:label>
        <rdfs:label xml:lang="sv">genomsnittligt antal lexikaliseringar</rdfs:label>
        <rdfs:isDefinedBy>http://www.w3.org/ns/lemon/lime</rdfs:isDefinedBy>
        <rdfs:comment xml:lang="en">The &apos;average number of lexicalizations&apos; property indicate the average number of lexicalizations per ontology element. The exact formula for calculating the average is indicated in the specification: https://www.w3.org/community/ontolex/wiki/Final_Model_Specification#LexicalizationSet</rdfs:comment>
        <rdfs:range rdf:resource="&xsd;decimal"/>
        <rdfs:domain rdf:resource="http://www.w3.org/ns/lemon/lime#LexicalizationSet"/>
    </owl:DatatypeProperty>
    


    <!-- http://www.w3.org/ns/lemon/lime#avgNumOfLinks -->

    <owl:DatatypeProperty rdf:about="http://www.w3.org/ns/lemon/lime#avgNumOfLinks">
        <rdfs:label xml:lang="de">Durchschnittliche Anzahl von Links</rdfs:label>
        <rdfs:label xml:lang="en">average number of links</rdfs:label>
        <rdfs:label xml:lang="es">promedio de enlaces</rdfs:label>
        <rdfs:label xml:lang="fr">nombre moyen de liens</rdfs:label>
        <rdfs:label xml:lang="it">numero medio di link</rdfs:label>
        <rdfs:label xml:lang="nl">gemiddeld aantal van links</rdfs:label>
        <rdfs:isDefinedBy>http://www.w3.org/ns/lemon/lime</rdfs:isDefinedBy>
        <rdfs:comment xml:lang="en">The &apos;average number of links&apos; property indicates the average number of links for each entity in the conceptual dataset.</rdfs:comment>
        <rdfs:range rdf:resource="&xsd;decimal"/>
        <rdfs:domain rdf:resource="http://www.w3.org/ns/lemon/lime#LexicalLinkset"/>
    </owl:DatatypeProperty>
    


    <!-- http://www.w3.org/ns/lemon/lime#avgSynonymy -->

    <owl:DatatypeProperty rdf:about="http://www.w3.org/ns/lemon/lime#avgSynonymy">
        <rdfs:label xml:lang="de">Durchschnittliche Synonymie</rdfs:label>
        <rdfs:label xml:lang="en">average synonymy</rdfs:label>
        <rdfs:label xml:lang="es">sinóminedad promedia</rdfs:label>
        <rdfs:label xml:lang="fr">synonymie moyenne</rdfs:label>
        <rdfs:label xml:lang="it">sinonimità media</rdfs:label>
        <rdfs:label xml:lang="nl">gemiddelde synonymie</rdfs:label>
        <rdfs:isDefinedBy>http://www.w3.org/ns/lemon/lime</rdfs:isDefinedBy>
        <rdfs:comment xml:lang="en">The &apos;average synonymy&apos; property indicates the average number of lexical entries evoking each lexical concept in the concept set.</rdfs:comment>
        <rdfs:range rdf:resource="&xsd;decimal"/>
        <rdfs:domain rdf:resource="http://www.w3.org/ns/lemon/lime#ConceptualizationSet"/>
    </owl:DatatypeProperty>
    


    <!-- http://www.w3.org/ns/lemon/lime#concepts -->

    <owl:DatatypeProperty rdf:about="http://www.w3.org/ns/lemon/lime#concepts">
        <rdfs:label xml:lang="de">Konzepte</rdfs:label>
        <rdfs:label xml:lang="en">concepts</rdfs:label>
        <rdfs:label xml:lang="es">conceptos</rdfs:label>
        <rdfs:label xml:lang="fr">concepts</rdfs:label>
        <rdfs:label xml:lang="it">concetti</rdfs:label>
        <rdfs:label xml:lang="nl">begrippen</rdfs:label>
        <rdfs:comment xml:lang="en">The &apos;concepts&apos; property indicates the number of lexical concepts defined in a concept set or involved in either a LexicalLinkset or ConceptualizationSet.</rdfs:comment>
        <rdfs:isDefinedBy xml:lang="en">http://www.w3.org/ns/lemon/lime</rdfs:isDefinedBy>
        <rdfs:range rdf:resource="&xsd;integer"/>
        <rdfs:domain>
            <owl:Class>
                <owl:unionOf rdf:parseType="Collection">
                    <rdf:Description rdf:about="http://www.w3.org/ns/lemon/lime#ConceptualizationSet"/>
                    <rdf:Description rdf:about="http://www.w3.org/ns/lemon/lime#LexicalLinkset"/>
                    <rdf:Description rdf:about="&ontolex;ConceptSet"/>
                </owl:unionOf>
            </owl:Class>
        </rdfs:domain>
    </owl:DatatypeProperty>
    


    <!-- http://www.w3.org/ns/lemon/lime#conceptualizations -->

    <owl:DatatypeProperty rdf:about="http://www.w3.org/ns/lemon/lime#conceptualizations">
        <rdfs:label xml:lang="de">Konzeptualisierungen</rdfs:label>
        <rdfs:label xml:lang="en">conceptualizations</rdfs:label>
        <rdfs:label xml:lang="es">conceptualizaciones</rdfs:label>
        <rdfs:label xml:lang="fr">conceptualisations</rdfs:label>
        <rdfs:label xml:lang="it">concettualizzazioni</rdfs:label>
        <rdfs:label xml:lang="nl">conceptualisaties</rdfs:label>
        <rdfs:isDefinedBy>http://www.w3.org/ns/lemon/lime</rdfs:isDefinedBy>
        <rdfs:comment xml:lang="en">The &apos;conceptualizations&apos; property indicates the number of distinct conceptualizations in a conceptualization set.</rdfs:comment>
        <rdfs:range rdf:resource="&xsd;integer"/>
        <rdfs:domain rdf:resource="http://www.w3.org/ns/lemon/lime#ConceptualizationSet"/>
    </owl:DatatypeProperty>
    


    <!-- http://www.w3.org/ns/lemon/lime#language -->

    <owl:DatatypeProperty rdf:about="http://www.w3.org/ns/lemon/lime#language">
        <rdfs:label xml:lang="af">taal</rdfs:label>
        <rdfs:label xml:lang="de">Sprache</rdfs:label>
        <rdfs:label xml:lang="en">language</rdfs:label>
        <rdfs:label xml:lang="es">lengua</rdfs:label>
        <rdfs:label xml:lang="fr">langue</rdfs:label>
        <rdfs:label xml:lang="it">lingua</rdfs:label>
        <rdfs:label xml:lang="nl">taal</rdfs:label>
        <rdfs:label xml:lang="pt">idioma</rdfs:label>
        <rdfs:label xml:lang="ro">limbă</rdfs:label>
        <rdfs:label xml:lang="sv">språk</rdfs:label>
        <rdfs:comment xml:lang="en">The  &apos;language&apos; property indicates the language of a lexicon, a lexical entry, a concept set or a lexicalization set.</rdfs:comment>
        <rdfs:isDefinedBy>http://www.w3.org/ns/lemon/lime</rdfs:isDefinedBy>
        <rdfs:range rdf:resource="&xsd;language"/>
        <rdfs:domain>
            <owl:Class>
                <owl:unionOf rdf:parseType="Collection">
                    <rdf:Description rdf:about="http://www.w3.org/ns/lemon/lime#LexicalizationSet"/>
                    <rdf:Description rdf:about="http://www.w3.org/ns/lemon/lime#Lexicon"/>
                    <rdf:Description rdf:about="&ontolex;ConceptSet"/>
                    <rdf:Description rdf:about="&ontolex;LexicalEntry"/>
                </owl:unionOf>
            </owl:Class>
        </rdfs:domain>
    </owl:DatatypeProperty>
    


    <!-- http://www.w3.org/ns/lemon/lime#lexicalEntries -->

    <owl:DatatypeProperty rdf:about="http://www.w3.org/ns/lemon/lime#lexicalEntries">
        <rdfs:label xml:lang="af">leksikale inskrywing</rdfs:label>
        <rdfs:label xml:lang="de">Lexikoneinträge</rdfs:label>
        <rdfs:label xml:lang="en">lexical entries</rdfs:label>
        <rdfs:label xml:lang="es">entradas léxicas</rdfs:label>
        <rdfs:label xml:lang="fr">lexie</rdfs:label>
        <rdfs:label xml:lang="it">entrate lessicali</rdfs:label>
        <rdfs:label xml:lang="nl">lexikaal items</rdfs:label>
        <rdfs:label xml:lang="pt">entradas lexicas</rdfs:label>
        <rdfs:label xml:lang="ro">înregistrari lexicale</rdfs:label>
        <rdfs:label xml:lang="sv">lexikoningångar</rdfs:label>
        <rdfs:isDefinedBy>http://www.w3.org/ns/lemon/lime</rdfs:isDefinedBy>
        <rdfs:comment xml:lang="en">The &apos;lexical entries&apos; property indicates the number of distinct lexical entries contained in a lexicon or lexicalization set.</rdfs:comment>
        <rdfs:range rdf:resource="&xsd;integer"/>
        <rdfs:isDefinedBy rdf:resource="http://www.w3.org/ns/lemon/lime"/>
        <rdfs:domain>
            <owl:Class>
                <owl:unionOf rdf:parseType="Collection">
                    <rdf:Description rdf:about="http://www.w3.org/ns/lemon/lime#ConceptualizationSet"/>
                    <rdf:Description rdf:about="http://www.w3.org/ns/lemon/lime#LexicalizationSet"/>
                    <rdf:Description rdf:about="http://www.w3.org/ns/lemon/lime#Lexicon"/>
                </owl:unionOf>
            </owl:Class>
        </rdfs:domain>
    </owl:DatatypeProperty>
    


    <!-- http://www.w3.org/ns/lemon/lime#lexicalizations -->

    <owl:DatatypeProperty rdf:about="http://www.w3.org/ns/lemon/lime#lexicalizations">
        <rdfs:label xml:lang="af">leksikaliserings</rdfs:label>
        <rdfs:label xml:lang="de">Lexikalisierungen</rdfs:label>
        <rdfs:label xml:lang="en">lexicalizations</rdfs:label>
        <rdfs:label xml:lang="es">lexicalizaciones</rdfs:label>
        <rdfs:label xml:lang="fr">lexicalisations</rdfs:label>
        <rdfs:label xml:lang="it">lessicalizzazioni</rdfs:label>
        <rdfs:label xml:lang="nl">lexicalisaties</rdfs:label>
        <rdfs:label xml:lang="pt">lexicalizações</rdfs:label>
        <rdfs:label xml:lang="ro">lexicalizari</rdfs:label>
        <rdfs:label xml:lang="sv">lexikaliseringar</rdfs:label>
        <rdfs:comment xml:lang="en">The &apos;lexicalizations&apos; property indicates the total number of lexicalizations in a lexicalization set, that is the number of unique pairs of lexical entry and denoted ontology element.</rdfs:comment>
        <rdfs:range rdf:resource="&xsd;integer"/>
        <rdfs:isDefinedBy rdf:resource="http://www.w3.org/ns/lemon/lime"/>
        <rdfs:domain rdf:resource="http://www.w3.org/ns/lemon/lime#LexicalizationSet"/>
    </owl:DatatypeProperty>
    


    <!-- http://www.w3.org/ns/lemon/lime#links -->

    <owl:DatatypeProperty rdf:about="http://www.w3.org/ns/lemon/lime#links">
        <rdfs:label xml:lang="de">Links</rdfs:label>
        <rdfs:label xml:lang="en">links</rdfs:label>
        <rdfs:label xml:lang="es">enlaces</rdfs:label>
        <rdfs:label xml:lang="fr">liens</rdfs:label>
        <rdfs:label xml:lang="it">link</rdfs:label>
        <rdfs:label xml:lang="nl">links</rdfs:label>
        <rdfs:comment xml:lang="en">The &apos;links&apos; property indicates the number of links between concepts in the concept set and entities in the reference dataset.</rdfs:comment>
        <rdfs:isDefinedBy>http://www.w3.org/ns/lemon/lime</rdfs:isDefinedBy>
        <rdfs:range rdf:resource="&xsd;integer"/>
        <rdfs:domain rdf:resource="http://www.w3.org/ns/lemon/lime#LexicalLinkset"/>
    </owl:DatatypeProperty>
    


    <!-- http://www.w3.org/ns/lemon/lime#percentage -->

    <owl:DatatypeProperty rdf:about="http://www.w3.org/ns/lemon/lime#percentage">
        <rdfs:label xml:lang="de">Prozentsatz</rdfs:label>
        <rdfs:label xml:lang="en">percentage</rdfs:label>
        <rdfs:label xml:lang="es">porcentaje</rdfs:label>
        <rdfs:label xml:lang="fr">pourcentage</rdfs:label>
        <rdfs:label xml:lang="it">percentuale</rdfs:label>
        <rdfs:label xml:lang="nl">percentage</rdfs:label>
        <rdfs:comment xml:lang="en">The &apos;percentage&apos; property expresses the percentage of entities in the reference dataset which have at least one lexicalization in a lexicalization set or are linked to a lexical concept in a lexical linkset.</rdfs:comment>
        <rdfs:isDefinedBy>http://www.w3.org/ns/lemon/lime</rdfs:isDefinedBy>
        <rdfs:range rdf:resource="&xsd;decimal"/>
        <rdfs:domain>
            <owl:Class>
                <owl:unionOf rdf:parseType="Collection">
                    <rdf:Description rdf:about="http://www.w3.org/ns/lemon/lime#LexicalLinkset"/>
                    <rdf:Description rdf:about="http://www.w3.org/ns/lemon/lime#LexicalizationSet"/>
                </owl:unionOf>
            </owl:Class>
        </rdfs:domain>
    </owl:DatatypeProperty>
    


    <!-- http://www.w3.org/ns/lemon/lime#references -->

    <owl:DatatypeProperty rdf:about="http://www.w3.org/ns/lemon/lime#references">
        <rdfs:label xml:lang="af">verwysings</rdfs:label>
        <rdfs:label xml:lang="de">Referenzen</rdfs:label>
        <rdfs:label xml:lang="en">references</rdfs:label>
        <rdfs:label xml:lang="es">referencias</rdfs:label>
        <rdfs:label xml:lang="fr">références</rdfs:label>
        <rdfs:label xml:lang="it">riferimenti</rdfs:label>
        <rdfs:label xml:lang="nl">referenties</rdfs:label>
        <rdfs:label xml:lang="pt">referencias</rdfs:label>
        <rdfs:label xml:lang="ro">referințe</rdfs:label>
        <rdfs:label xml:lang="sv">referenser</rdfs:label>
        <rdfs:comment xml:lang="en">The &apos;references&apos; property indicates the number of distinct ontology or vocabulary elements that are either associated with lexical entries via a lexicalization set or linked to lexical concepts via a lexical link set.</rdfs:comment>
        <rdfs:range rdf:resource="&xsd;integer"/>
        <rdfs:isDefinedBy rdf:resource="http://www.w3.org/ns/lemon/lime"/>
        <rdfs:domain>
            <owl:Class>
                <owl:unionOf rdf:parseType="Collection">
                    <rdf:Description rdf:about="http://www.w3.org/ns/lemon/lime#LexicalLinkset"/>
                    <rdf:Description rdf:about="http://www.w3.org/ns/lemon/lime#LexicalizationSet"/>
                </owl:unionOf>
            </owl:Class>
        </rdfs:domain>
    </owl:DatatypeProperty>
    


    <!-- 
    ///////////////////////////////////////////////////////////////////////////////////////
    //
    // Classes
    //
    ///////////////////////////////////////////////////////////////////////////////////////
     -->

    


    <!-- http://rdfs.org/ns/void#Dataset -->

    <owl:Class rdf:about="&void;Dataset"/>
    


    <!-- http://rdfs.org/ns/void#Linkset -->

    <owl:Class rdf:about="&void;Linkset"/>
    


    <!-- http://www.w3.org/2000/01/rdf-schema#Class -->

    <owl:Class rdf:about="&rdfs;Class"/>
    


    <!-- http://www.w3.org/ns/lemon/lime#ConceptualizationSet -->

    <owl:Class rdf:about="http://www.w3.org/ns/lemon/lime#ConceptualizationSet">
        <rdfs:label xml:lang="de">Konzeptualisierungsatz</rdfs:label>
        <rdfs:label xml:lang="en">conceptualization set</rdfs:label>
        <rdfs:label xml:lang="es">conjuto de conceptualizaciones</rdfs:label>
        <rdfs:label xml:lang="fr">banque de concepitalisations</rdfs:label>
        <rdfs:label xml:lang="it">banca concettualizzazioni</rdfs:label>
        <rdfs:label xml:lang="nl">verzameling van conceptialisaties</rdfs:label>
        <rdfs:subClassOf rdf:resource="&void;Dataset"/>
        <rdfs:subClassOf>
            <owl:Restriction>
                <owl:onProperty rdf:resource="http://www.w3.org/ns/lemon/lime#conceptualDataset"/>
                <owl:onClass rdf:resource="&ontolex;ConceptSet"/>
                <owl:qualifiedCardinality rdf:datatype="&xsd;nonNegativeInteger">1</owl:qualifiedCardinality>
            </owl:Restriction>
        </rdfs:subClassOf>
        <rdfs:subClassOf>
            <owl:Restriction>
                <owl:onProperty rdf:resource="http://www.w3.org/ns/lemon/lime#lexiconDataset"/>
                <owl:onClass rdf:resource="http://www.w3.org/ns/lemon/lime#Lexicon"/>
                <owl:qualifiedCardinality rdf:datatype="&xsd;nonNegativeInteger">1</owl:qualifiedCardinality>
            </owl:Restriction>
        </rdfs:subClassOf>
        <rdfs:comment xml:lang="en">A conceptualization set represents a collection of links between lexical entries in a Lexicon and lexical concepts in a Concept Set they evoke.</rdfs:comment>
        <rdfs:isDefinedBy>http://www.w3.org/ns/lemon/lime</rdfs:isDefinedBy>
    </owl:Class>
    


    <!-- http://www.w3.org/ns/lemon/lime#LexicalLinkset -->

    <owl:Class rdf:about="http://www.w3.org/ns/lemon/lime#LexicalLinkset">
        <rdfs:label xml:lang="af">leksikale skakelstel</rdfs:label>
        <rdfs:label xml:lang="de">Lexikonlinksatz</rdfs:label>
        <rdfs:label xml:lang="en">lexical linkset</rdfs:label>
        <rdfs:label xml:lang="es">conjunto de enlaces</rdfs:label>
        <rdfs:label xml:lang="fr">banque de liens lexicals</rdfs:label>
        <rdfs:label xml:lang="it">banca di link lessicali</rdfs:label>
        <rdfs:label xml:lang="nl">verzameling van lexicale links</rdfs:label>
        <rdfs:label xml:lang="ro">linkset lexical</rdfs:label>
        <rdfs:label xml:lang="sv">lexikalisk länkmängd</rdfs:label>
        <rdfs:subClassOf rdf:resource="&void;Linkset"/>
        <rdfs:subClassOf>
            <owl:Restriction>
                <owl:onProperty rdf:resource="http://www.w3.org/ns/lemon/lime#conceptualDataset"/>
                <owl:onClass rdf:resource="&ontolex;ConceptSet"/>
                <owl:qualifiedCardinality rdf:datatype="&xsd;nonNegativeInteger">1</owl:qualifiedCardinality>
            </owl:Restriction>
        </rdfs:subClassOf>
        <rdfs:subClassOf>
            <owl:Restriction>
                <owl:onProperty rdf:resource="http://www.w3.org/ns/lemon/lime#referenceDataset"/>
                <owl:onClass rdf:resource="&void;Dataset"/>
                <owl:qualifiedCardinality rdf:datatype="&xsd;nonNegativeInteger">1</owl:qualifiedCardinality>
            </owl:Restriction>
        </rdfs:subClassOf>
        <rdfs:subClassOf>
            <owl:Restriction>
                <owl:onProperty rdf:resource="http://www.w3.org/ns/lemon/lime#partition"/>
                <owl:allValuesFrom rdf:resource="http://www.w3.org/ns/lemon/lime#LexicalLinkset"/>
            </owl:Restriction>
        </rdfs:subClassOf>
        <rdfs:comment xml:lang="en">A lexical linkset represents a collection of links between a reference dataset and a set of lexical concepts (e.g. synsets of a wordnet).</rdfs:comment>
        <rdfs:isDefinedBy rdf:resource="http://www.w3.org/ns/lemon/lime"/>
    </owl:Class>
    


    <!-- http://www.w3.org/ns/lemon/lime#LexicalizationSet -->

    <owl:Class rdf:about="http://www.w3.org/ns/lemon/lime#LexicalizationSet">
        <rdfs:label xml:lang="en">lexicalization set</rdfs:label>
        <rdfs:subClassOf rdf:resource="&void;Dataset"/>
        <rdfs:subClassOf>
            <owl:Restriction>
                <owl:onProperty rdf:resource="http://www.w3.org/ns/lemon/lime#referenceDataset"/>
                <owl:onClass rdf:resource="&void;Dataset"/>
                <owl:qualifiedCardinality rdf:datatype="&xsd;nonNegativeInteger">1</owl:qualifiedCardinality>
            </owl:Restriction>
        </rdfs:subClassOf>
        <rdfs:subClassOf>
            <owl:Restriction>
                <owl:onProperty rdf:resource="http://www.w3.org/ns/lemon/lime#partition"/>
                <owl:allValuesFrom rdf:resource="http://www.w3.org/ns/lemon/lime#LexicalizationSet"/>
            </owl:Restriction>
        </rdfs:subClassOf>
        <rdfs:subClassOf>
            <owl:Restriction>
                <owl:onProperty rdf:resource="http://www.w3.org/ns/lemon/lime#lexicalizationModel"/>
                <owl:cardinality rdf:datatype="&xsd;nonNegativeInteger">1</owl:cardinality>
            </owl:Restriction>
        </rdfs:subClassOf>
        <rdfs:subClassOf>
            <owl:Restriction>
                <owl:onProperty rdf:resource="http://www.w3.org/ns/lemon/lime#lexiconDataset"/>
                <owl:onClass rdf:resource="http://www.w3.org/ns/lemon/lime#Lexicon"/>
                <owl:maxQualifiedCardinality rdf:datatype="&xsd;nonNegativeInteger">1</owl:maxQualifiedCardinality>
            </owl:Restriction>
        </rdfs:subClassOf>
        <rdfs:comment xml:lang="en">A &apos;lexicalization set&apos; is a dataset that comprises a collection of lexicalizations, that is pairs of lexical entry and corresponding reference in the associated ontology/vocabulary/dataset.</rdfs:comment>
        <rdfs:isDefinedBy rdf:resource="http://www.w3.org/ns/lemon/lime"/>
    </owl:Class>
    


    <!-- http://www.w3.org/ns/lemon/lime#Lexicon -->

    <owl:Class rdf:about="http://www.w3.org/ns/lemon/lime#Lexicon">
        <rdfs:label xml:lang="af">leksikon</rdfs:label>
        <rdfs:label xml:lang="de">Lexikon</rdfs:label>
        <rdfs:label xml:lang="en">lexicon</rdfs:label>
        <rdfs:label xml:lang="es">lexicón</rdfs:label>
        <rdfs:label xml:lang="fr">Lexique</rdfs:label>
        <rdfs:label xml:lang="it">Lessico</rdfs:label>
        <rdfs:label xml:lang="nl">Lexicon</rdfs:label>
        <rdfs:label xml:lang="ro">lexicon</rdfs:label>
        <rdfs:label xml:lang="sv">lexikon</rdfs:label>
        <rdfs:subClassOf rdf:resource="&void;Dataset"/>
        <rdfs:subClassOf>
            <owl:Restriction>
                <owl:onProperty rdf:resource="http://www.w3.org/ns/lemon/lime#entry"/>
                <owl:onClass rdf:resource="&ontolex;LexicalEntry"/>
                <owl:minQualifiedCardinality rdf:datatype="&xsd;nonNegativeInteger">1</owl:minQualifiedCardinality>
            </owl:Restriction>
        </rdfs:subClassOf>
        <rdfs:subClassOf>
            <owl:Restriction>
                <owl:onProperty rdf:resource="http://www.w3.org/ns/lemon/lime#language"/>
                <owl:cardinality rdf:datatype="&xsd;nonNegativeInteger">1</owl:cardinality>
            </owl:Restriction>
        </rdfs:subClassOf>
        <rdfs:isDefinedBy>http://www.w3.org/ns/lemon/lime</rdfs:isDefinedBy>
        <rdfs:comment xml:lang="en">A lexicon represents a collection of lexical entries for a particular language or domain.</rdfs:comment>
    </owl:Class>
    


    <!-- 
    ///////////////////////////////////////////////////////////////////////////////////////
    //
    // Annotations
    //
    ///////////////////////////////////////////////////////////////////////////////////////
     -->

    <rdf:Description rdf:about="http://www.w3.org/ns/lemon/lime#lexicalizationModel">
        <rdfs:label xml:lang="de">Lexikalisierungmodell</rdfs:label>
        <rdfs:label xml:lang="en">lexicalization model</rdfs:label>
        <rdfs:label xml:lang="es">modelo de lexicalización</rdfs:label>
        <rdfs:label xml:lang="fr">modèle de lexicalisation</rdfs:label>
        <rdfs:label xml:lang="it">modello di lessicalizzazione</rdfs:label>
        <rdfs:label xml:lang="nl">model van lexicalisatie</rdfs:label>
        <rdfs:comment xml:lang="en">The &apos;lexicalization model&apos; property indicates the model used for representing lexical information. Possible values include (but are not limited to) http://www.w3.org/2000/01/rdf-schema# (for the use of rdfs:label), http://www.w3.org/2004/02/skos/core (for the use of skos:pref/alt/hiddenLabel), http://www.w3.org/2008/05/skos-xl (for the use of skosxl:pref/alt/hiddenLabel) and http://www.w3.org/ns/lemon/all for lemon.</rdfs:comment>
        <rdfs:isDefinedBy>http://www.w3.org/ns/lemon/lime</rdfs:isDefinedBy>
    </rdf:Description>
</rdf:RDF>



<!-- Generated by the OWL API (version 3.5.1) http://owlapi.sourceforge.net -->

